dumps/proof_producing_nat_comparisons.lean
@@ -1,6 +1,0 @@
-import Init.Prelude
-
-def castComparison
-    (h : Nat.blt 99999999 100000000 = true) :
-    Nat.ble 100000000 100000000 = true :=
-  h
